checked_add proof

Generated/erc20shim/ERC20Shim/Common/switch_2364266820542243941_user.lean
@@ -15,12 +15,66 @@ section
 
 open Clear EVMState Ast Expr Stmt FunctionDefinition State Interpreter ExecLemmas OutOfFuelLemmas Abstraction YulNotation PrimOps ReasoningPrinciple Utilities ERC20Shim.Common Generated.erc20shim ERC20Shim
 
-def A_switch_2364266820542243941 (s₀ s₉ : State) : Prop := sorry
+def A_switch_2364266820542243941 (s₀ s₉ : State) : Prop :=
+  s₉.isOk ∧
+
+  (--Case 1: No initial collision
+    s₀.evm.hash_collision = false →
+  (
+    ( -- Case 1.1 : _3 = 0
+      (-- Case 1.1.1: _7 = 1 (Reversion)
+        preservesEvm s₀ s₉ ∧
+        s₉.evm.reverted = true ∧
+        s₉.evm.hash_collision = false
+      )
+      ∨
+      (-- Case 1.1.2 _7 =/ 0 (Non Reversion)
+        preservesEvm s₀ s₉ ∧
+        s₉.evm.hash_collision = false
+      )
+    )
+    ∨
+    ( -- Case 1.2 : Default
+      preservesEvm s₀ s₉ ∧
+      s₉.evm.hash_collision = false
+    )
+    ∨
+      -- Case 1.3 : Collision in function
+      s₉.evm.hash_collision = true
+  )
+  )
+  ∧
+  (-- Case 2: existing initial collision
+     s₀.evm.hash_collision = true →
+    s₉.evm.hash_collision = true
+  )
+
+set_option maxHeartbeats 2000000
 
 lemma switch_2364266820542243941_abs_of_concrete {s₀ s₉ : State} :
   Spec switch_2364266820542243941_concrete_of_code s₀ s₉ →
   Spec A_switch_2364266820542243941 s₀ s₉ := by
-  sorry
+
+  unfold switch_2364266820542243941_concrete_of_code A_switch_2364266820542243941
+
+  rcases s₀ with ⟨evm₀, varstore₀⟩ | _ | _ <;> [simp only; aesop_spec; aesop_spec]
+
+  apply spec_eq
+
+  rintro hasFuel ⟨s1, call_mapping1,
+                  ⟨s2, call_308,
+                    ⟨s3, call_mapping2,
+                      ⟨s4, call_update1,
+                        ⟨s5, call_add,
+                          ⟨s6, call_update2, code⟩⟩⟩⟩⟩⟩
+
+  generalize s0_all :
+  (Ok evm₀ varstore₀) = s₀ at *
+
+  unfold A_mapping_index_access_mapping_address_uint256_of_address at call_mapping1
+  unfold lookup! State.insert at call_mapping1
+  simp[←s0_all] at call_mapping1
+
 
 end
 
