Generated/erc20shim/ERC20Shim/checked_add_uint256_user.lean
@@ -12,13 +12,147 @@ section
 
 open Clear EVMState Ast Expr Stmt FunctionDefinition State Interpreter ExecLemmas OutOfFuelLemmas Abstraction YulNotation PrimOps ReasoningPrinciple Utilities ERC20Shim.Common Generated.erc20shim ERC20Shim
 
-def A_checked_add_uint256 (sum : Identifier) (x y : Literal) (s₀ s₉ : State) : Prop := sorry
+def A_checked_add_uint256 (sum : Identifier) (x y : Literal) (s₀ s₉ : State) : Prop :=
+  s₉.isOk ∧
+
+  (--Case 1: No initial collision
+    s₀.evm.hash_collision = false →
+  (
+    ( -- Case 1.1 : Reversion
+      preservesEvm s₀ s₉ ∧
+      s₉.evm.reverted = true ∧
+      x > s₉[sum]!! ∧
+      s₉.evm.hash_collision = false
+    )
+    ∨
+    ( -- Case 1.2 : No Reversion
+      preservesEvm s₀ s₉ ∧
+      x ≤ s₉[sum]!! ∧
+      s₉.evm.hash_collision = false
+    )
+    ∨
+      -- Case 1.3 : Collision in function
+      s₉.evm.hash_collision = true
+  )
+  )
+  ∧
+  (-- Case 2: existing initial collision
+     s₀.evm.hash_collision = true →
+    s₉.evm.hash_collision = true
+  )
+
+set_option maxHeartbeats 1000000
 
 lemma checked_add_uint256_abs_of_concrete {s₀ s₉ : State} {sum x y} :
   Spec (checked_add_uint256_concrete_of_code.1 sum x y) s₀ s₉ →
   Spec (A_checked_add_uint256 sum x y) s₀ s₉ := by
+
   unfold checked_add_uint256_concrete_of_code A_checked_add_uint256
-  sorry
+  rcases s₀ with ⟨evm₀, varstore₀⟩ | _ | _ <;> [simp only; aesop_spec; aesop_spec]
+  apply spec_eq
+  clr_funargs
+  clr_varstore,
+  rintro hasFuel ⟨s, call_if, code⟩
+
+  generalize sinhab_all :
+  (Ok evm₀ Inhabited.default⟦"y"↦y⟧⟦"x"↦x⟧⟦"x"↦x⟧⟦"y"↦y⟧⟦"sum"↦x + y⟧⟦"_1"↦(decide (x + y < x)).toUInt256⟧)
+  = sinhab at *
+
+  generalize s0_all :
+  (Ok evm₀ varstore₀) = s₀ at *
+
+  have s0_sinhab_preservesEvm : preservesEvm s₀ sinhab := by
+    unfold preservesEvm
+    simp [←s0_all, ←sinhab_all]
+    unfold State.insert
+    simp
+
+  unfold A_if_2792370840247009933 at call_if
+  clr_spec at call_if
+
+  obtain ⟨s_ok, s_no_collision, s_collision⟩ := call_if
+
+  obtain ⟨s_evm, ⟨s_varstore, s_all⟩⟩ := State_of_isOk s_ok
+
+  unfold reviveJump at code
+  simp [←s0_all, s_all] at code
+
+  by_cases collision_s0 : s₀.evm.hash_collision = false
+
+  · -- no collision at s₀
+    have : sinhab.evm.hash_collision = false := by aesop
+    simp[this] at s_no_collision
+
+    obtain ⟨sinhab_s_preservesEvm, mstore, reversion, store_eq, s_no_collision⟩ |
+            ⟨sinhab_s_preservesEvm, reversion, s_store, s_no_collision⟩ |
+            collision_s := s_no_collision
+    · -- Reverted
+      have : ¬sinhab["_1"]!! = 0 → (decide (x + y < x)).toUInt256 ≠ 0 := by
+        simp
+        unfold lookup!
+        simp[←sinhab_all]
+        unfold State.insert
+        simp
+
+      have : (decide (x + y < x)).toUInt256 ≠ 0 → x + y < x := by
+        unfold Bool.toUInt256
+        simp
+
+      split_ands
+      · aesop
+      · simp[collision_s0]
+        left
+        split_ands
+        · aesop
+        · aesop
+        · unfold lookup!
+          simp[←code]
+          unfold lookup!
+          simp
+          unfold State.insert at sinhab_all
+          simp at sinhab_all
+          have : s_varstore = (Finmap.insert "_1" (decide (x + y < x)).toUInt256
+                                (Finmap.insert "sum" (x + y)
+                                  (Finmap.insert "y" y (Finmap.insert "x" x (Finmap.insert "y" y Inhabited.default))))) := by aesop
+          simp[this]
+          aesop
+        · aesop
+      · aesop
+    · -- Not Reverted
+
+      have h1 : sinhab["_1"]!! = 0 → (decide (x + y < x)).toUInt256 = 0 := by
+        simp
+        unfold lookup!
+        simp[←sinhab_all]
+        unfold State.insert
+        simp
+
+      have h2 : (decide (x + y < x)).toUInt256 = 0 → x ≤ x + y := by
+        unfold Bool.toUInt256
+        simp
+
+      split_ands
+      · aesop
+      · simp[collision_s0]
+        right
+        left
+        split_ands
+        · aesop
+        · rw[←code]
+          unfold lookup!
+          simp
+          unfold State.insert at sinhab_all
+          simp at sinhab_all
+          have : s_varstore = (Finmap.insert "_1" (decide (x + y < x)).toUInt256
+                                (Finmap.insert "sum" (x + y)
+                                  (Finmap.insert "y" y (Finmap.insert "x" x (Finmap.insert "y" y Inhabited.default))))) := by aesop
+          simp[this]
+          have : x ≤ x + y := by aesop
+          aesop
+        · aesop
+      · aesop
+    · aesop
+  · aesop
 
 end
 
